WIP

code/ecdsa/Hacl.Impl.EC.Exponent.fst
@@ -31,19 +31,41 @@ open Hacl.Impl.P521.Exponent
 open Hacl.Impl.EC.Setup
 
 open Hacl.Impl.MM.Exponent
+open Lib.ByteSequence 
+
+#set-options "--z3rlimit 100 --ifuel 0 --fuel 0"
+
+val lemma_list_nat_from_bytes: a: list uint8 { List.Tot.length a <= max_size_t} -> 
+  i: nat {i > 0 /\ i <= List.Tot.length a} ->
+  Lemma (Lib.ByteSequence.nat_from_intseq_le (Lib.Sequence.slice (Lib.Sequence.of_list a) 0 i) == lst_as_nat_ a i)
+
+let rec lemma_list_nat_from_bytes a i = 
+  let l = List.Tot.length a in 
+  let al = (Lib.Sequence.of_list a) in 
+  let sl = (Lib.Sequence.slice al 0 i) in 
+  match i with 
+  |1 -> nat_from_intseq_le_lemma0 sl; lst_as_nat_first a
+  |_ -> lemma_list_nat_from_bytes a (i - 1);
+    let i1 = i - 1 in 
+    nat_from_intseq_le_slice_lemma al i1;
+    nat_from_intseq_le_slice_lemma sl (i - 1);
+    nat_from_intseq_le_lemma0 (Lib.Sequence.slice sl i1 i); 
+    lst_as_nat_definiton a i
+
 
 
 let exponent #c a result tempBuffer = 
   match c with 
-  |P256 -> 
-    exponent_p256 a result tempBuffer
-  |P384 ->
-    exponent_p384 a result tempBuffer
-  |Default -> 
+  |P256 -> exponent_p256 a result tempBuffer
+  |P384 -> exponent_p384 a result tempBuffer
+  |_ -> 
     recall_contents (prime_inverse_buffer #c) (Lib.Sequence.of_list (prime_inverse_list c));
-    montgomery_ladder_power #c #DH a (prime_inverse_buffer #c) result
+    montgomery_ladder_power #c #DH a (prime_inverse_buffer #c) result;
+    lemma_list_nat_from_bytes (prime_inverse_list c) (List.Tot.length (prime_inverse_list c))
 
 
 let square_root #c a result = 
   recall_contents (sqPower_buffer #c) (Lib.Sequence.of_list (sqPower_list #c));
-  montgomery_ladder_power #c #DH a (sqPower_buffer #c) result
+  montgomery_ladder_power #c #DH a (sqPower_buffer #c) result;
+  lemma_list_nat_from_bytes (sqPower_list #c) (List.Tot.length (sqPower_list #c))
+
