code/ecdsa/Hacl.Impl.P384.Exponent.fsti
@@ -1,0 +1,23 @@
+module Hacl.Impl.P384.Exponent
+
+open FStar.HyperStack.All
+open FStar.HyperStack
+module ST = FStar.HyperStack.ST
+
+open Lib.IntTypes
+open Lib.Buffer
+
+open Hacl.Spec.EC.Definition
+open Spec.ECC
+open Spec.ECC.Curves
+open Hacl.Spec.MontgomeryMultiplication
+
+
+val exponent_p384: a: felem P384 -> result: felem P384 -> 
+  tempBuffer: lbuffer uint64 (getCoordinateLenU64 P384 *. 8ul) -> Stack unit
+  (requires fun h -> live h a /\ live h tempBuffer /\ live h result /\ disjoint tempBuffer result /\ 
+    disjoint a tempBuffer /\ as_nat P384 h a < getPrime P384)
+  (ensures fun h0 _ h1 -> modifies (loc result |+| loc tempBuffer) h0 h1 /\ (
+    let k = fromDomain_ #P384 #DH (as_nat P384 h0 a) in 
+    as_nat P384 h1 result =  toDomain_ #P384 #DH (pow k (prime384 - 2) % prime384) /\
+    as_nat P384 h1 result < getPrime P384)) 
